Valaig/ForLean/Function.lean
@@ -1,0 +1,13 @@
+module
+
+public section
+
+theorem hfunext {α α' : Sort u} {β : α → Sort v} {β' : α' → Sort v} {f : ∀ a, β a} {f' : ∀ a, β' a}
+    (hα : α = α') (h : ∀ a a', a ≍ a' → f a ≍ f' a') : f ≍ f' := by
+  subst hα
+  have : ∀ a, f a ≍ f' a := fun a ↦ h a a (HEq.refl a)
+  have : β = β' := by funext a; exact type_eq_of_heq (this a)
+  subst this
+  grind
+
+end
